feat : completeness of LJFPS

src/rules/Measures.v
@@ -1,8 +1,5 @@
 From Equations Require Import Equations.
 From Stdlib Require Import List.
-
-From CARVe Require Import contexts.list.   
-From CARVe Require algebras.dill algebras.structural.  
 From LJF Require Import SharedLogic.
 
 Equations osize (A : o) : nat :=
@@ -12,11 +9,11 @@ Equations osize (A : o) : nat :=
   osize (AndP A B) := 1 + osize A + osize B;
   osize (AndN A B) := 1 + osize A + osize B;
   osize (Or   A B) := 1 + osize A + osize B;
-  osize (Impl A B) := 1 + osize A + osize B
+  osize (Imp A B) := 1 + osize A + osize B
 .
-
-Equations octx_size (O: octx) : nat :=
+About osize_equation_1.
+Equations octx_size (L: octx) : nat :=
     octx_size nil := 0;
-    octx_size (A :: O') := osize A + octx_size O'
+    octx_size (A :: L') := osize A + octx_size L'
 .
 
