src/metatheory/LJFPS_Exchange.v
@@ -1,10 +1,8 @@
 From Equations Require Import Equations.
-From Stdlib Require Import List.
-From CARVe Require Import contexts.list.
-From CARVe Require Import algebras.structural.
-From LJF Require Import SharedLogic LJFPS_Rules.
-From Stdlib Require Import Permutation.
+From Stdlib Require Import List Permutation.
+From Stdlib Require Import Wellfounded Nat Arith Lia.
 
+From LJF Require Import SharedLogic Measures LJFPS_Rules.
 
 Scheme bct_mut := Induction for bct Sort Prop
   with ept_mut := Induction for ept Sort Prop
@@ -13,65 +11,59 @@ Scheme bct_mut := Induction for bct Sort Prop
 
 Combined Scheme LJFPS_mutind_all from bct_mut, ept_mut, lfc_mut, rfc_mut.
 
-Theorem LJFPS_exchange_structural_perm :
-  (forall {C: sctx} {D: octx} {K: o}, bct C D K -> forall {C': sctx}, Permutation C C' -> bct C' D K) /\
-  (forall {C: sctx} {D: octx} {K: o}, ept C D K -> forall {C': sctx}, Permutation C C' -> ept C' D K) /\
+Theorem LJFPS_exchange_structural :
+  (forall {C: sctx} {L: octx} {K: o}, bct C L K -> forall {C': sctx}, Permutation C C' -> bct C' L K) /\
+  (forall {C: sctx} {L: octx} {K: o}, ept C L K -> forall {C': sctx}, Permutation C C' -> ept C' L K) /\
   (forall {C: sctx} {N K: o}, lfc C N K -> forall {C': sctx}, Permutation C C' -> lfc C' N K) /\
   (forall {C: sctx} {P: o}, rfc C P -> forall {C': sctx}, Permutation C C' -> rfc C' P). 
 Proof.
     apply LJFPS_mutind_all ; intros.
-        - apply bct_R_box. apply b. apply H. apply H0.
-        - apply bct_R_AndN. 
-            + apply H. apply H1.
-            + apply H0. apply H1.
-        - apply bct_R_Impl. apply H. apply H0.
-        - apply ept_L_f with (N := N). apply b. apply n. apply perm_has_entry with (l := S).
-            apply h. apply H0. apply H. apply H0.
-        - apply ept_R_f. apply p. apply H. apply H0.
-        - apply ept_L_box. apply b. apply p. apply H. apply Permutation_cons. 
-            reflexivity. apply H0.
-        - apply ept_L_AndP. apply b. apply H. apply H0.
-        - apply ept_L_Or. apply b. apply H. apply H1. apply H0. apply H1.
-        - apply ept_L_True. apply b. apply H. apply H0.
-        - apply ept_L_False. apply b.
-        - apply lfc_R_l. apply b. apply p. apply H. apply H0.
-        - apply lfc_I_l. apply n. apply a.
-        - apply lfc_L_AndN_1. apply b. apply H. apply H0.
-        - apply lfc_L_AndN_2. apply b. apply H. apply H0.
-        - apply lfc_L_Impl. apply b. apply H. apply H1. apply H0. apply H1.
-        - apply rfc_R_r. apply n. apply H. apply H0.
-        - apply rfc_I_r. apply p. apply a. apply perm_has_entry with (l := S).
-            apply h. apply H.
-        - apply rfc_R_AndP. apply H. apply H1. apply H0. apply H1.
-        - apply rfc_R_Or_1. apply H. apply H0.
-        - apply rfc_R_Or_2. apply H. apply H0.
-        - apply rfc_R_True.
+        - apply bct_boxR. apply b. apply H. apply H0.
+        - apply bct_AndNR. apply H. apply H1. apply H0. apply H1.
+        - apply bct_ImpR. apply H. apply H0.
+        - eapply ept_Lf. eapply Permutation_in. apply H0. apply i. apply b. apply n. apply H. apply H0.
+        - apply ept_Rf. apply p. apply H. apply H0.
+        - apply ept_boxL. apply b. apply p. apply H. apply Permutation_cons. reflexivity. apply H0.
+        - apply ept_AndPL. apply b. apply H. apply H0.
+        - apply ept_OrL. apply b. apply H. apply H1. apply H0. apply H1.
+        - apply ept_TrueL. apply b. apply H. apply H0.
+        - apply ept_FalseL. apply b.
+        - apply lfc_Rl. apply b. apply p. apply H. apply H0.
+        - apply lfc_Il. apply n. apply a.
+        - apply lfc_AndNL_1. apply b. apply H. apply H0.
+        - apply lfc_AndNL_2. apply b. apply H. apply H0.
+        - apply lfc_ImpL. apply b. apply H. apply H1. apply H0. apply H1.
+        - apply rfc_Rr. apply n. apply H. apply H0.
+        - apply rfc_Ir. eapply Permutation_in. apply H. apply i. apply p. apply a.
+        - apply rfc_AndPR. apply H. apply H1. apply H0. apply H1.
+        - apply rfc_OrR_1. apply H. apply H0.
+        - apply rfc_OrR_2. apply H. apply H0.
+        - apply rfc_TrueR.
 Qed.
 
-Lemma LJFPS_exchange_structural_perm_bct :
-    forall {C: sctx} {D: octx} {K: o}, bct C D K -> forall {C': sctx}, Permutation C C' -> bct C' D K.
+Lemma LJFPS_exchange_structural_bct :
+    forall {C: sctx} {L: octx} {K: o}, bct C L K -> forall {C': sctx}, Permutation C C' -> bct C' L K.
 Proof.
-  destruct LJFPS_exchange_structural_perm. apply H.
+  destruct LJFPS_exchange_structural. apply H.
 Qed.
 
-Lemma LJFPS_exchange_structural_perm_ept :
-    forall {C: sctx} {D: octx} {K: o}, ept C D K -> forall {C': sctx}, Permutation C C' -> ept C' D K.
+Lemma LJFPS_exchange_structural_ept :
+    forall {C: sctx} {L: octx} {K: o}, ept C L K -> forall {C': sctx}, Permutation C C' -> ept C' L K.
 Proof.
-  destruct LJFPS_exchange_structural_perm. destruct H0. apply H0.
+  destruct LJFPS_exchange_structural. destruct H0. apply H0.
 Qed.
 
-Lemma LJFPS_exchange_structural_perm_lfc :
+Lemma LJFPS_exchange_structural_lfc :
   forall {C: sctx} {N K: o}, lfc C N K -> forall {C': sctx}, Permutation C C' -> lfc C' N K.
 Proof.
-  destruct LJFPS_exchange_structural_perm. destruct H0. destruct H1. apply H1.
+  destruct LJFPS_exchange_structural. destruct H0. destruct H1. apply H1.
 Qed.
 
-Lemma LJFPS_exchange_structural_perm_rfc :
+Lemma LJFPS_exchange_structural_rfc :
   forall {C: sctx} {K: o}, rfc C K -> forall {C': sctx}, Permutation C C' -> rfc C' K.
 Proof.
-  destruct LJFPS_exchange_structural_perm. destruct H0. destruct H1. apply H2.
+  destruct LJFPS_exchange_structural. destruct H0. destruct H1. apply H2.
 Qed.
-
 
 Lemma Permutation_singleton : 
   forall {B: o} {C: octx},
@@ -84,318 +76,326 @@ Proof.
     - transitivity l'. apply IHPermutation2. symmetry. transitivity l. symmetry. apply Heqb.
       symmetry. apply IHPermutation1. apply Heqb. apply IHPermutation1. apply Heqb.
 Qed.
-  
 
-Lemma LJFPS_eager_box :
-  forall {S': sctx} {O: octx} {K: o}, 
+Lemma eager_boxL :
+  forall {C0: sctx} {L: octx} {B: o} {K: o},
     bracketable K ->
-    ept S' O K ->
-  forall {S: sctx} {B: o},
-    Permutation S' ((B, tt) :: S) ->
     permeable B ->
-    forall {O1 O2: octx}, 
-    O = O1 ++ O2 ->
-    ept S (O1 ++ B :: O2) K.
+    ept C0 L K ->
+    forall {C: sctx} {L1 L2: octx},
+      Permutation C0 (B :: C) ->
+      L = L1 ++ L2 ->
+      ept C (L1 ++ B :: L2) K.
 Proof.
-  intros S' O K Br H. induction H ; intros S0 B0 Pt Pb O1 O2 Ho.
-    - symmetry in Ho. apply app_eq_nil in Ho. destruct Ho. subst.
-      simpl. apply ept_L_box. apply H. apply Pb.
-      apply ept_L_f with (N := N). apply H. apply H0.
-        + apply perm_has_entry with (l := S). apply H1. apply Pt.
-        + eapply LJFPS_exchange_structural_perm_lfc. apply H2. apply Pt.
-    - symmetry in Ho. apply app_eq_nil in Ho. destruct Ho. subst.
-      simpl. apply ept_L_box. apply Br. apply Pb.
-      apply ept_R_f. apply H. eapply LJFPS_exchange_structural_perm_rfc.
-      apply H0. apply Pt.
-    - symmetry in Ho. apply app_eq_cons in Ho. destruct Ho.
-      + destruct H2. subst. simpl. 
-        apply ept_L_box. apply Br. apply Pb.
-        apply ept_L_box. apply Br. apply H0.
-        eapply LJFPS_exchange_structural_perm_ept. apply H1. apply Permutation_cons.
-        reflexivity. apply Pt.
-      + destruct H2. destruct H2. subst. simpl.
-        apply ept_L_box. apply H. apply H0.
-        eapply IHept. apply Br. apply Permutation_sym. 
-        -- apply perm_trans with ((B, tt) :: (B0, tt) :: S0). apply perm_swap.
-           apply Permutation_cons. reflexivity. apply Permutation_sym. apply Pt.
-        -- apply Pb.
-        -- reflexivity.
-    - symmetry in Ho. apply app_eq_cons in Ho. destruct Ho.
-      + destruct H1. subst. simpl.
-        apply ept_L_box. apply H. apply Pb.
-        apply ept_L_AndP. apply H.
-        eapply LJFPS_exchange_structural_perm_ept. apply H0. apply Pt.
-      + destruct H1. destruct H1. subst. simpl.
-        apply ept_L_AndP. apply H.
-        eapply IHept with (O1 := B2 :: B1 :: x). apply Br. apply Pt. apply Pb. reflexivity.
-    - symmetry in Ho. apply app_eq_cons in Ho. destruct Ho.
+  intros C0 L B K b p H ; induction H ; intros.
+    - symmetry in H4. apply app_eq_nil in H4. destruct H4. subst. simpl.
+      apply ept_boxL. apply b. apply p.
+      eapply ept_Lf. eapply Permutation_in. apply H3. apply H. apply b. apply H1.
+      eapply LJFPS_exchange_structural_lfc. apply H2. apply H3.
+    - symmetry in H2. apply app_eq_nil in H2. destruct H2. subst. simpl.
+      apply ept_boxL. apply b. apply p.
+      apply ept_Rf. apply H. 
+      eapply LJFPS_exchange_structural_rfc. apply H0. apply H1.
+    - symmetry in H3. apply app_eq_cons in H3. destruct H3. 
+      + destruct H3. subst. simpl.
+        apply ept_boxL. apply b. apply p. 
+        eapply LJFPS_exchange_structural_ept. 2: apply H2.
+        apply ept_boxL. apply H. apply H0. apply H1.
+      + destruct H3. destruct H3. subst. simpl. 
+        apply ept_boxL. apply H. apply H0.
+        apply IHept. apply H.
+        assert (Permutation (B :: B0 :: C0) (B0 :: B :: C0)). apply perm_swap.
+        apply Permutation_sym in H3. eapply perm_trans.
+          -- apply perm_skip with (x := B0)  in H2. apply H2.
+          -- apply H3.
+          -- reflexivity.
+    - symmetry in H2. apply app_eq_cons in H2. destruct H2 ; destruct H2.
+      + subst. simpl. apply ept_boxL. apply b. apply p.
+        apply ept_AndPL. apply b.
+        eapply LJFPS_exchange_structural_ept. apply H0. apply H1.
       + destruct H2. subst. simpl.
-        apply ept_L_box. apply H. apply Pb.
-        apply ept_L_Or. apply H.
-        -- eapply LJFPS_exchange_structural_perm_ept. apply H0. apply Pt.
-        -- eapply LJFPS_exchange_structural_perm_ept. apply H1. apply Pt.
-      + destruct H2. destruct H2. subst. simpl.
-        apply ept_L_Or. apply H.
-        -- eapply IHept1 with (O1 := B1 :: x). apply Br. apply Pt. apply Pb. reflexivity. 
-        -- eapply IHept2 with (O1 := B2 :: x). apply Br. apply Pt. apply Pb. reflexivity. 
-    - symmetry in Ho. apply app_eq_cons in Ho. destruct Ho.
+        apply ept_AndPL. apply H.
+        eapply IHept with (L1 := B2 :: B1 :: x). apply b. apply H1. reflexivity.
+    - symmetry in H3. apply app_eq_cons in H3. destruct H3 ; destruct H3.
+      + subst. simpl.
+        apply ept_boxL. apply b. apply p.
+        apply ept_OrL. apply b.
+          -- eapply LJFPS_exchange_structural_ept. apply H0. apply H2.
+          -- eapply LJFPS_exchange_structural_ept. apply H1. apply H2.
+      + destruct H3. subst. simpl. 
+        apply ept_OrL. apply b.
+          -- eapply IHept1 with (L1 := B1 :: x). apply b. apply H2. reflexivity.
+          -- eapply IHept2 with (L1 := B2 :: x). apply b. apply H2. reflexivity.
+    - symmetry in H2. apply app_eq_cons in H2. destruct H2 ; destruct H2.
+      + subst. simpl. apply ept_boxL. apply b. apply p.
+        apply ept_TrueL. apply b.
+        eapply LJFPS_exchange_structural_ept. apply H0. apply H1.
+      + destruct H2. subst. simpl.
+        apply ept_TrueL. apply H.
+        eapply IHept with (L1 := x). apply b. apply H1. reflexivity.
+    - symmetry in H1. apply app_eq_cons in H1. destruct H1 ; destruct H1.
+      + subst. simpl. apply ept_boxL. apply b. apply p.
+        apply ept_FalseL. apply b.
       + destruct H1. subst. simpl.
-        apply ept_L_box. apply H. apply Pb.
-        apply ept_L_True. apply H. 
-        eapply LJFPS_exchange_structural_perm_ept. apply H0. apply Pt.
-      + destruct H1. destruct H1. subst. simpl.
-        apply ept_L_True. apply H.
-        eapply IHept. apply Br. apply Pt. apply Pb. reflexivity.
-    - symmetry in Ho. apply app_eq_cons in Ho. destruct Ho.
-      + destruct H0. subst. simpl. 
-        apply ept_L_box. apply H. apply Pb. apply ept_L_False. apply H.
-      + destruct H0. destruct H0. subst. simpl. apply ept_L_False. apply H.
-Qed.
-
-Lemma LJFPS_eager_AndP :
-  forall {S: sctx} {O: octx} {K: o},
+        apply ept_FalseL. apply H.
+Qed.        
+        
+Lemma eager_AndPL :
+  forall {C: sctx} {L: octx} {B1 B2 K: o},
     bracketable K ->
-    ept S O K ->
-    forall {B1 B2: o} {O1 O2: octx},
-      O = O1 ++ B2 :: B1 :: O2 ->
-      ept S (O1 ++ (AndP B1 B2) :: O2) K.
+    ept C L K ->
+      forall {L1 L2: octx},
+      L = L1 ++ B2 :: B1 :: L2 ->
+      ept C (L1 ++ (AndP B1 B2) :: L2) K.
 Proof.
-  intros S O K Br H. induction H ; intros B1' B2' O1 O2 Ho.
+  intros C L B1 B2 K b H. induction H ; intros L1 L2 Ho.
     - symmetry in Ho. apply app_eq_nil in Ho. destruct Ho. discriminate H4.
     - symmetry in Ho. apply app_eq_nil in Ho. destruct Ho. discriminate H2.
     - symmetry in Ho. apply app_eq_cons in Ho. destruct Ho.
       + destruct H2. inversion H3. subst. clear H3. simpl.
-        apply ept_L_AndP. apply H.
-        apply ept_L_box. apply H. apply H0. apply H1. 
+        apply ept_AndPL. apply H.
+        apply ept_boxL. apply H. apply H0. apply H1. 
       + destruct H2. destruct H2. subst. simpl.
-        apply ept_L_box. apply H. apply H0. 
+        apply ept_boxL. apply H. apply H0. 
         apply IHept. apply H. reflexivity.
     - symmetry in Ho. apply app_eq_cons in Ho. destruct Ho.
       + destruct H1. inversion H2. subst. simpl.
-        apply ept_L_AndP. apply H. 
-        apply ept_L_AndP. apply H. apply H0. 
+        apply ept_AndPL. apply H. 
+        apply ept_AndPL. apply H. apply H0. 
       + destruct H1. destruct H1. subst. simpl.
-        apply ept_L_AndP. apply H.
-        eapply IHept with (O1 := (B2 :: B1 :: x)). apply H. reflexivity.
+        apply ept_AndPL. apply H.
+        apply IHept with (L1 := B3 :: B0 :: x). apply b. reflexivity.
     - symmetry in Ho. apply app_eq_cons in Ho. destruct Ho.
       + destruct H2. inversion H3. subst. simpl. clear H3.
-        apply ept_L_AndP. apply H. apply ept_L_Or. apply H.
-        apply H0. apply H1.
+        apply ept_AndPL. apply H. 
+        apply ept_OrL. apply H. apply H0. apply H1.
       + destruct H2. destruct H2. subst. simpl.
-        apply ept_L_Or. apply H.
-        -- apply IHept1 with (O1 := (B1 :: x)). apply H. reflexivity.
-        -- apply IHept2 with (O1 := (B2 :: x)). apply H. reflexivity.
+        apply ept_OrL. apply H.
+        -- apply IHept1 with (L1 := (B0 :: x)). apply H. reflexivity.
+        -- apply IHept2 with (L1 := (B3 :: x)). apply H. reflexivity.
     - symmetry in Ho. apply app_eq_cons in Ho. destruct Ho.
       + destruct H1. inversion H2. subst. simpl.
-        apply ept_L_AndP. apply H.
-        apply ept_L_True. apply H.
+        apply ept_AndPL. apply H.
+        apply ept_TrueL. apply H.
         apply H0.
       + destruct H1. destruct H1. subst. simpl.
-        apply ept_L_True. apply H. 
+        apply ept_TrueL. apply H. 
         apply IHept. apply H. reflexivity.
     - symmetry in Ho. apply app_eq_cons in Ho. destruct Ho.
       + destruct H0. inversion H1. subst. simpl. 
-        apply ept_L_AndP. apply H. apply ept_L_False. apply H.
+        apply ept_AndPL. apply H. apply ept_FalseL. apply H.
       + destruct H0. destruct H0. subst. simpl.
-        apply ept_L_False. apply H.
+        apply ept_FalseL. apply H.
 Qed.
 
-Lemma LJFPS_eager_True :
-  forall {S: sctx} {O: octx} {K: o},
-    bracketable K ->
-    ept S O K ->
-    forall {O1 O2: octx},
-      O = O1 ++ O2 ->
-      ept S (O1 ++ TT :: O2) K.
-Proof.
-  intros S O K Br H. induction H ; intros O0 O3 Ho.
-    - symmetry in Ho. apply app_eq_nil in Ho. destruct Ho. subst. simpl.
-      apply ept_L_True. apply H. eapply ept_L_f. apply H. apply H0.
-      apply H1. apply H2.
-    - symmetry in Ho. apply app_eq_nil in Ho. destruct Ho. subst. simpl.
-      apply ept_L_True. apply Br. apply ept_R_f. apply H. apply H0.
-    - destruct O0.
-      + simpl in Ho. subst. simpl. apply ept_L_True. apply H.
-        apply ept_L_box. apply H. apply H0. apply H1.
-      + simpl in Ho. inversion Ho. subst. simpl.
-        apply ept_L_box. apply H. apply H0.
-        apply IHept. apply H. reflexivity.
-    - destruct O0.
-      + simpl in Ho. subst. simpl. apply ept_L_True. apply H.
-        apply ept_L_AndP. apply H. apply H0.
-      + simpl in Ho. inversion Ho. subst. simpl.
-        apply ept_L_AndP. apply H.
-        eapply IHept with (O1 := B2 :: B1 :: O0) (O2 := O3). apply H. reflexivity.
-    - destruct O0.
-      + simpl in Ho. subst. simpl. apply ept_L_True. apply H.
-        apply ept_L_Or. apply H. apply H0. apply H1.
-      + simpl in Ho. inversion Ho. subst. simpl.
-        apply ept_L_Or. apply H.
-        -- eapply IHept1 with (O1 := B1 :: O0). apply H. reflexivity.
-        -- eapply IHept2 with (O1 := B2 :: O0). apply H. reflexivity.
-    - destruct O0.
-      + simpl in Ho. subst. simpl. apply ept_L_True. apply H.
-        apply ept_L_True. apply H. apply H0.
-      + simpl in Ho. inversion Ho. subst. simpl.
-        apply ept_L_True. apply H. apply IHept. apply H. reflexivity.
-    - destruct O0.
-      + simpl in Ho. subst. simpl. apply ept_L_True. apply H.
-        apply ept_L_False. apply H.
-      + simpl in Ho. inversion Ho. subst. simpl.
-        apply ept_L_False. apply H.
-Qed.
-
-
-Lemma LJFPS_inversion_L_box :
-  forall {S: sctx} {O: octx} {B K: o},
+Lemma LJFPS_inversion_boxL :
+  forall {C: sctx} {L: octx} {B K: o},
     bracketable K ->
     permeable B ->
-    ept S O K ->
-    forall {O': octx},
-      O = B :: O' ->  
-      ept ((B, tt) :: S) O' K.
+    ept C L K ->
+    forall {L1: octx},
+      L = B :: L1 ->  
+      ept (B :: C) L1 K.
 Proof.
-  intros S O B K Br Pb H. induction H ; intros O1 Ho.
+  intros C L B K b p H. induction H ; intros L1 Ho.
     - discriminate Ho.
     - discriminate Ho.
     - inversion Ho. subst. apply H1.
-    - inversion Ho. subst. inversion Pb. inversion H1. inversion H1.
-    - inversion Ho. subst. inversion Pb. inversion H2. inversion H2.
-    - inversion Ho. subst. inversion Pb. inversion H1. inversion H1.
-    - inversion Ho. subst. inversion Pb. inversion H0. inversion H0.
+    - inversion Ho. subst. inversion p. inversion H1. inversion H1.
+    - inversion Ho. subst. inversion p. inversion H2. inversion H2.
+    - inversion Ho. subst. inversion p. inversion H1. inversion H1.
+    - inversion Ho. subst. inversion p. inversion H0. inversion H0.
 Qed.
 
-Lemma LJFPS_eager_Or :
-  forall {S: sctx} {O: octx} {K: o},
+Lemma eager_OrL :
+  forall {C: sctx} {L: octx} {B1 B2 K: o},
     bracketable K ->
-    ept S O K ->
-    forall {O' : octx},
-      ept S O' K ->
-      forall {B1 B2: o} {O1 O2: octx},
-        O = O1 ++ B1 :: O2 ->
-        O' = O1 ++ B2 :: O2 ->
-        ept S (O1 ++ (Or B1 B2) :: O2) K.
+    ept C L K ->
+    forall {L' : octx},
+      ept C L' K ->
+      forall {L1 L2: octx},
+        L = L1 ++ B1 :: L2 ->
+        L' = L1 ++ B2 :: L2 ->
+        ept C (L1 ++ (Or B1 B2) :: L2) K.
 Proof.
-  intros S O K Br H. induction H ; intros O' H' B0 B3 O1 O2 Ho Ho'.
+  intros C L B1 B2 K b H. induction H ; intros L' H' L1 L2 Ho Ho'.
     - subst. symmetry in Ho. apply app_eq_nil in Ho. destruct Ho.
       inversion H4.
     - subst. symmetry in Ho. apply app_eq_nil in Ho. destruct Ho.
       inversion H2.
     - subst. symmetry in Ho. apply app_eq_cons in Ho. destruct Ho.
       + destruct H2. inversion H3. subst. simpl. 
-        apply ept_L_Or. apply H.
-          -- apply ept_L_box. apply H. apply H0. apply H1.
+        apply ept_OrL. apply H.
+          -- apply ept_boxL. apply H. apply H0. apply H1.
           -- apply H'.
       + destruct H2. destruct H2. subst. simpl.
-        apply ept_L_box. apply H. apply H0.
+        apply ept_boxL. apply H. apply H0.
         simpl in H'.
-        eapply IHept with (O' := x ++ B3 :: O2). apply H.
-        eapply LJFPS_inversion_L_box. apply H. apply H0.
+        eapply IHept with (L' := x ++ B2 :: L2). apply H.
+        eapply LJFPS_inversion_boxL. apply H. apply H0.
         apply H'. reflexivity. reflexivity. reflexivity.
     - symmetry in Ho. apply app_eq_cons in Ho. destruct Ho.
       + destruct H1. inversion H2. subst. simpl. 
-        apply ept_L_Or. apply H. apply ept_L_AndP. apply H. apply H0. apply H'.
+        apply ept_OrL. apply H. apply ept_AndPL. apply H. apply H0. apply H'.
       + destruct H1. destruct H1. subst.
-        simpl. apply ept_L_AndP. apply H.
-        eapply IHept with (O1 := B2 :: B1 :: x). apply H.
+        simpl. apply ept_AndPL. apply H.
+        eapply IHept with (L1 := B3 :: B0 :: x). apply H.
         inversion H'. subst. inversion H5. inversion H1. inversion H1. subst.
         apply H7. reflexivity. reflexivity.
     - subst. symmetry in Ho. apply app_eq_cons in Ho. destruct Ho.
       + destruct H2. inversion H3. subst. simpl.
-        apply ept_L_Or. apply H. apply ept_L_Or. apply H.
+        apply ept_OrL. apply H. apply ept_OrL. apply H.
         apply H0. apply H1. apply H'.
       + destruct H2. destruct H2. subst. simpl.
-        apply ept_L_Or. apply H. 
+        apply ept_OrL. apply H. 
         inversion H'. subst. inversion H6. inversion H2. inversion H2. subst.
-        eapply IHept1 with (O1 := B1 :: x). apply H. apply H8. reflexivity. reflexivity.
+        eapply IHept1 with (L1 := B0 :: x). apply H. apply H8. reflexivity. reflexivity.
         inversion H'. subst. inversion H6. inversion H2. inversion H2. subst.
-        eapply IHept2 with (O1 := B2 :: x). apply H. apply H9. reflexivity. reflexivity.
+        eapply IHept2 with (L1 := B3 :: x). apply H. apply H9. reflexivity. reflexivity.
     - symmetry in Ho. apply app_eq_cons in Ho. destruct Ho.
       + destruct H1. inversion H2. subst. simpl.
-        apply ept_L_Or. apply H.
-        apply ept_L_True. apply H. apply H0.
+        apply ept_OrL. apply H.
+        apply ept_TrueL. apply H. apply H0.
         apply H'.
       + destruct H1. destruct H1. subst. simpl.
-        apply ept_L_True. apply H.
+        apply ept_TrueL. apply H.
         eapply IHept. apply H.
         inversion H'. subst. inversion H5. inversion H1. inversion H1.
         subst. apply H4. reflexivity. reflexivity.
     - symmetry in Ho. apply app_eq_cons in Ho. destruct Ho.
       + destruct H0. inversion H1. subst. simpl.
-        apply ept_L_Or. apply H. apply ept_L_False. apply H. apply H'.
-      + destruct H0. destruct H0. subst. simpl. apply ept_L_False. apply H.
+        apply ept_OrL. apply H. apply ept_FalseL. apply H. apply H'.
+      + destruct H0. destruct H0. subst. simpl. apply ept_FalseL. apply H.
 Qed. 
 
-
-Lemma LJFPS_eager_False :
-  forall {O1: octx} {K: o},
+Lemma eager_TrueL :
+  forall {C: sctx} {L: octx} {K: o},
     bracketable K ->
-    forall {S: sctx} {O2: octx},
-    ept S (O1 ++ FF :: O2) K.
-Admitted.
+    ept C L K ->
+    forall {L1 L2: octx},
+      L = L1 ++ L2 ->
+      ept C (L1 ++ TT :: L2) K.
+Proof.
+  intros C L K b H. induction H ; intros L1 L2 Ho.
+    - symmetry in Ho. apply app_eq_nil in Ho. destruct Ho. subst. simpl.
+      apply ept_TrueL. apply b. eapply ept_Lf. apply H. apply H0.
+      apply H1. apply H2.
+    - symmetry in Ho. apply app_eq_nil in Ho. destruct Ho. subst. simpl.
+      apply ept_TrueL. apply b. apply ept_Rf. apply H. apply H0.
+    - destruct L1.
+      + simpl in Ho. subst. simpl. apply ept_TrueL. apply H.
+        apply ept_boxL. apply H. apply H0. apply H1.
+      + simpl in Ho. inversion Ho. subst. simpl.
+        apply ept_boxL. apply H. apply H0.
+        apply IHept. apply H. reflexivity.
+    - destruct L1.
+      + simpl in Ho. subst. simpl. apply ept_TrueL. apply H.
+        apply ept_AndPL. apply H. apply H0.
+      + simpl in Ho. inversion Ho. subst. simpl.
+        apply ept_AndPL. apply H.
+        eapply IHept with (L1 := B2 :: B1 :: L1) (L2 := L2). apply H. reflexivity.
+    - destruct L1.
+      + simpl in Ho. subst. simpl. apply ept_TrueL. apply H.
+        apply ept_OrL. apply H. apply H0. apply H1.
+      + simpl in Ho. inversion Ho. subst. simpl.
+        apply ept_OrL. apply H.
+        -- eapply IHept1 with (L1 := B1 :: L1). apply H. reflexivity.
+        -- eapply IHept2 with (L1 := B2 :: L1). apply H. reflexivity.
+    - destruct L1.
+      + simpl in Ho. subst. simpl. apply ept_TrueL. apply H.
+        apply ept_TrueL. apply H. apply H0.
+      + simpl in Ho. inversion Ho. subst. simpl.
+        apply ept_TrueL. apply H. apply IHept. apply H. reflexivity.
+    - destruct L1.
+      + simpl in Ho. subst. simpl. apply ept_TrueL. apply H.
+        apply ept_FalseL. apply H.
+      + simpl in Ho. inversion Ho. subst. simpl.
+        apply ept_FalseL. apply H.
+Qed.
 
+Lemma eager_FalseL : 
+  forall {C: sctx} {L: octx} {K: o},
+    bracketable K ->
+    In FF L ->
+    ept C L K.
+Proof.
+  intros C L K b. revert C.
+  induction L using (well_founded_ind (wf_inverse_image octx nat lt octx_size PeanoNat.Nat.lt_wf_0)).
+  destruct L ; intros C I. inversion I. destruct o.
+    + apply ept_boxL. apply b. destruct p. 
+      apply Permeable_pos_atom. apply Is_atom. apply Pos_atom.
+      apply Permeable_neg. apply Neg_atom. apply H.
+      simp octx_size. inversion I. discriminate H0. apply H0.
+    + apply ept_TrueL. apply b. apply H.
+      simp octx_size. inversion I. discriminate H0. apply H0.
+    + apply ept_FalseL. apply b.
+    + apply ept_AndPL. apply b. apply H.
+      simp octx_size. simp osize.
+      simpl. rewrite Nat.add_shuffle3. rewrite Nat.add_assoc. apply Nat.lt_succ_diag_r.
+      inversion I. discriminate H0. apply in_cons. apply in_cons. apply H0.
+    + apply ept_boxL. apply b. apply Permeable_neg. apply Neg_and.
+      apply H. simp octx_size. apply Nat.lt_add_pos_l. 
+      simp osize. apply Nat.lt_lt_add_r. apply Nat.lt_lt_add_r. apply Nat.lt_0_1.
+      inversion I. discriminate H0. apply H0.
+    + apply ept_OrL. apply b.
+      -- apply H. simp octx_size. simp osize. simpl.
+        apply Nat.lt_succ_r.
+        apply add_le_mono_r_proj_l2r. apply Nat.le_add_r.
+        inversion I. discriminate H0. apply in_cons. apply H0.
+      -- apply H. simp octx_size. simp osize. simpl.
+        apply Nat.lt_succ_r.
+        apply add_le_mono_r_proj_l2r. apply Nat.le_add_l.
+        inversion I. discriminate H0. apply in_cons. apply H0.
+    + apply ept_boxL. apply b. apply Permeable_neg. apply Neg_imp.
+      apply H. simp octx_size. apply Nat.lt_add_pos_l. 
+      simp osize. apply Nat.lt_lt_add_r. apply Nat.lt_lt_add_r. apply Nat.lt_0_1.
+      inversion I. discriminate H0. apply H0.
+Qed.
 
 Scheme bct_mut_async := Induction for bct Sort Prop
   with ept_mut_async := Induction for ept Sort Prop.
 Combined Scheme LJFPS_mutind_async from bct_mut_async, ept_mut_async.
 
-Lemma LJF_exchange_ordered_perm :
-  (forall {C: sctx} {D: octx} {K: o}, bct C D K -> forall {D': octx}, Permutation D D' -> bct C D' K) /\
-  (forall {C: sctx} {D: octx} {K: o}, ept C D K -> forall {D': octx}, Permutation D D' -> ept C D' K).
+Lemma LJFPS_exchange_ordered_perm :
+  (forall {C: sctx} {L: octx} {K: o}, bct C L K -> forall {L': octx}, Permutation L L' -> bct C L' K) /\
+  (forall {C: sctx} {L: octx} {K: o}, ept C L K -> forall {L': octx}, Permutation L L' -> ept C L' K).
 Proof.
     apply LJFPS_mutind_async ; intros.
-        - apply bct_R_box. apply b. apply H. apply H0.
-        - apply bct_R_AndN. apply H. apply H1. apply H0. apply H1.
-        - apply bct_R_Impl. apply H. apply Permutation_cons. reflexivity. apply H0.
-        - apply Permutation_nil in H. subst. apply ept_L_f with (N := N) ; assumption.
-        - apply Permutation_nil in H. subst. apply ept_R_f ; assumption.
-        - assert (Hin : In B D').
-          + apply Permutation_in with (x := B) in H0. apply H0. apply in_eq.  
-          + apply in_split in Hin. destruct Hin. destruct H1. subst.
-            eapply LJFPS_eager_box.
-            -- apply b.
-            -- apply H. eapply Permutation_cons_app_inv. apply H0.
-            -- apply Permutation_refl.
-            -- apply p.
-            -- reflexivity.
-        - assert (Hin : In (AndP B1 B2) D').
-          + apply Permutation_in with (x := (AndP B1 B2)) in H0. apply H0. apply in_eq.
-          + apply in_split in Hin. destruct Hin. destruct H1. subst.
-            eapply LJFPS_eager_AndP. apply b. 
-            assert (H1 : ept S (x ++ B2 :: B1 :: x0) K).
-            apply H. 
-            apply Permutation_cons_app_inv with (l := O) in H0.
-            apply Permutation_cons_app with (l := B1 :: O).
-            apply Permutation_cons_app with (l := O). apply H0.
-            apply H1. reflexivity.   
-        - assert (Hin : In (Or B1 B2) D').
-          + apply Permutation_in with (x := Or B1 B2) in H1. apply H1. apply in_eq.
-          + apply in_split in Hin. destruct Hin. destruct H2. subst.
-            eapply LJFPS_eager_Or. apply b.
-            assert (H2 : ept S (x ++ B1 :: x0) K).
-            apply H. 
-            eapply Permutation_cons_app_inv with (l := O) in H1.
-            eapply Permutation_cons_app with (l := O). apply H1.
-            apply H2.
-            assert (H2 : ept S (x ++ B2 :: x0) K).
-            apply H0. 
-            eapply Permutation_cons_app_inv with (l := O) in H1.
-            eapply Permutation_cons_app with (l := O). apply H1.
-            apply H2.
-            reflexivity. reflexivity.
-        - assert (Hin : In TT D').
-          + apply Permutation_in with (x := TT) in H0. apply H0. apply in_eq.
-          + apply in_split in Hin. destruct Hin. destruct H1. subst.
-            eapply LJFPS_eager_True. apply b.
-            assert (H1 : ept S (x ++ x0) K).
-            apply H. 
-            eapply Permutation_cons_app_inv with (l := O) in H0.
-            apply H0.
-            apply H1.
-            reflexivity.
-        - assert (Hin : In FF D').
-          + apply Permutation_in with (x := FF) in H. apply H. apply in_eq.
-          + apply in_split in Hin. destruct Hin. destruct H0. subst.
-            eapply LJFPS_eager_False. apply b.
+      - apply bct_boxR. apply b. apply H. apply H0.
+      - apply bct_AndNR. apply H. apply H1. apply H0. apply H1.
+      - apply bct_ImpR. apply H. apply Permutation_cons. reflexivity. apply H0.
+      - apply Permutation_nil in H. subst. eapply ept_Lf. apply i. apply b. apply n. apply l.
+      - apply Permutation_nil in H. subst. apply ept_Rf. apply p. apply r.
+      - pose proof H0.
+        symmetry in H1. apply Permutation_vs_cons_inv in H1. destruct H1. destruct H1. subst.
+        eapply eager_boxL. apply b. apply p. 3: reflexivity. 2: apply Permutation_refl.
+        apply H. eapply Permutation_cons_app_inv. apply H0.
+      - pose proof H0.
+        symmetry in H1. apply Permutation_vs_cons_inv in H1. destruct H1. destruct H1. subst.
+        eapply eager_AndPL. apply b. 2: reflexivity.
+        apply H. apply Permutation_cons_app. apply Permutation_cons_app. eapply Permutation_cons_app_inv. apply H0.
+      - pose proof H1.
+        symmetry in H1. apply Permutation_vs_cons_inv in H1. destruct H1. destruct H1. subst.
+        eapply eager_OrL. apply b. 4: reflexivity. 3:reflexivity.
+          + apply H. apply Permutation_cons_app. eapply Permutation_cons_app_inv. apply H2.
+          + apply H0. apply Permutation_cons_app. eapply Permutation_cons_app_inv. apply H2.
+      - pose proof H0.
+        symmetry in H1. apply Permutation_vs_cons_inv in H1. destruct H1. destruct H1. subst.
+        eapply eager_TrueL. apply b. 2: reflexivity.
+        apply H. eapply Permutation_cons_app_inv. apply H0. 
+      - apply eager_FalseL. apply b. apply Permutation_in with (x:= FF) in H.
+        apply H. apply in_eq.
+Qed.
+
+Lemma LJFPS_exchange_ordered_perm_bct :
+  forall {C: sctx} {L: octx} {K: o}, bct C L K -> forall {L': octx}, Permutation L L' -> bct C L' K.
+Proof.
+  destruct LJFPS_exchange_ordered_perm. apply H.
+Qed.
+
+Lemma LJFPS_exchange_ordered_perm_ept :
+  forall {C: sctx} {L: octx} {K: o}, ept C L K -> forall {L': octx}, Permutation L L' -> ept C L' K.
+Proof.
+  destruct LJFPS_exchange_ordered_perm. apply H0.
 Qed.
 
